feat: test file operators (-f -d -e -s -r -w -x)

c/coreutils.c
@@ -147,3 +147,4 @@ LEAN_EXPORT lean_object *lean_coreutils_nanosleep(uint64_t ns, lean_object *w) {
     }
     return lean_io_result_mk_ok(lean_box_uint64(0));
 }
+
